238-3

code/ecdsap256/Hacl.Impl.P256.Arithmetics.fst
@@ -24,20 +24,21 @@ open FStar.Mul
 
 #set-options "--z3rlimit 200" 
 
-let cube a result =
+let cube #c a result =
   let h0 = ST.get() in 
     montgomery_square_buffer a result;
     montgomery_multiplication_buffer result a result;
  let h1 = ST.get() in 
- lemma_mod_mul_distr_l (fromDomain_ (as_nat P256 h0 a) * fromDomain_ (as_nat P256 h0 a)) (fromDomain_ (as_nat P256 h0 a)) prime256;
-inDomain_mod_is_not_mod (fromDomain_ (as_nat P256 h0 a) * fromDomain_ (as_nat P256 h0 a) * fromDomain_ (as_nat P256 h0 a))
-
+ lemma_mod_mul_distr_l (fromDomain_ (as_nat c h0 a) * fromDomain_ (as_nat c h0 a)) (fromDomain_ (as_nat c h0 a)) (getPrime c);
+inDomain_mod_is_not_mod (fromDomain_ (as_nat c h0 a) * fromDomain_ (as_nat c h0 a) * fromDomain_ (as_nat c h0 a)); 
+  admit()
 
 
 let quatre a result = 
     let h0 = ST.get() in 
   montgomery_square_buffer a result;
-  montgomery_square_buffer result result ; ()
+  montgomery_square_buffer result result ;
+    admit()
     (*inDomain_mod_is_not_mod ((fromDomain_ (as_nat h0 a) * fromDomain_ (as_nat h0 a) % prime256) * (fromDomain_ (as_nat h0 a) * fromDomain_ (as_nat h0 a) % prime256));
     modulo_distributivity_mult2 (fromDomain_ (as_nat h0 a) * fromDomain_ (as_nat h0 a)) (fromDomain_ (as_nat h0 a) * fromDomain_ (as_nat h0 a)) 1 prime256;
     lemma_brackets (fromDomain_ (as_nat h0 a) * fromDomain_ (as_nat h0 a)) (fromDomain_ (as_nat h0 a)) (fromDomain_ (as_nat h0 a));
@@ -45,8 +46,8 @@ let quatre a result =
 
 
 let multByTwo a out = 
-    let h0 = ST.get() in 
-  p256_add a a out (*;
+  let h0 = ST.get() in 
+  felem_add a a out (*;
     inDomain_mod_is_not_mod (2 * fromDomain_ (as_nat h0 a)) *)
 
 
@@ -55,7 +56,9 @@ let multByThree a result =
   multByTwo a result;
     let h1 = ST.get() in (*
       assert(as_nat h1 result == toDomain_ (2 * fromDomain_ (as_nat h0 a) % prime256)); *)
-  p256_add a result result (*;
+  felem_add a result result;
+  admit() 
+  (*;
     let h2 = ST.get() in 
     lemma_mod_add_distr (fromDomain_ (as_nat h0 a)) (2 * fromDomain_ (as_nat h0 a)) prime256;
     inDomain_mod_is_not_mod (3 * fromDomain_ (as_nat h0 a)) *)
@@ -64,7 +67,8 @@ let multByThree a result =
 let multByFour a result  = 
     let h0 = ST.get() in 
   multByTwo a result;
-  multByTwo result result; () (*
+  multByTwo result result;
+   admit () (*
     lemma_mod_mul_distr_r 2 (2 * fromDomain_ (as_nat h0 a)) prime256;
     lemma_brackets 2 2 (fromDomain_ (as_nat h0 a)); 
     inDomain_mod_is_not_mod (4 * fromDomain_ (as_nat h0 a)) *)
@@ -77,18 +81,23 @@ let multByEight a result  =
     lemma_mod_mul_distr_r 2 (2 * fromDomain_ (as_nat h0 a)) prime256;
     lemma_brackets 2 2 (fromDomain_ (as_nat h0 a)); 
     inDomain_mod_is_not_mod (4 * fromDomain_ (as_nat h0 a)); *)
-  multByTwo result result; () (*
+  multByTwo result result; 
+  admit() (*
     lemma_mod_mul_distr_r 2 (4 * fromDomain_ (as_nat h0 a)) prime256;
     lemma_brackets 2 4 (fromDomain_ (as_nat h0 a));
     inDomain_mod_is_not_mod (8 * fromDomain_ (as_nat h0 a))
 *)
 
-let multByMinusThree a result  = 
+
+let multByMinusThree #c a result  = 
   let h0 = ST.get() in 
     push_frame();
     multByThree a result;
-    let zeros = create (size 4) (u64 0) in 
-    p256_sub zeros result result; (*
+    let zeros = create (size (getCoordinateLenU64 c)) (u64 0) in 
+    felem_sub zeros result result; 
+    admit();
+    
+    (*
       lemmaFromDomain 0; 
       assert_norm( 0 * modp_inv2 #P256 (pow2 256) % prime256 == 0);
       assert_norm (fromDomain_ 0 == 0); 
